misc tuning and modernization;

src/HOL/Isar_Examples/Expr_Compiler.thy
@@ -10,20 +10,17 @@ theory Expr_Compiler
 imports Main
 begin
 
-text {*
- This is a (rather trivial) example of program verification.  We model
- a compiler for translating expressions to stack machine instructions,
- and prove its correctness wrt.\ some evaluation semantics.
-*}
+text {* This is a (rather trivial) example of program verification.
+  We model a compiler for translating expressions to stack machine
+  instructions, and prove its correctness wrt.\ some evaluation
+  semantics. *}
 
 
 subsection {* Binary operations *}
 
-text {*
- Binary operations are just functions over some type of values.  This
- is both for abstract syntax and semantics, i.e.\ we use a ``shallow
- embedding'' here.
-*}
+text {* Binary operations are just functions over some type of values.
+  This is both for abstract syntax and semantics, i.e.\ we use a
+  ``shallow embedding'' here. *}
 
 types
   'val binop = "'val => 'val => 'val"
@@ -31,85 +28,71 @@ types
 
 subsection {* Expressions *}
 
-text {*
- The language of expressions is defined as an inductive type,
- consisting of variables, constants, and binary operations on
- expressions.
-*}
+text {* The language of expressions is defined as an inductive type,
+  consisting of variables, constants, and binary operations on
+  expressions. *}
 
 datatype ('adr, 'val) expr =
-  Variable 'adr |
-  Constant 'val |
-  Binop "'val binop" "('adr, 'val) expr" "('adr, 'val) expr"
+    Variable 'adr
+  | Constant 'val
+  | Binop "'val binop" "('adr, 'val) expr" "('adr, 'val) expr"
 
-text {*
- Evaluation (wrt.\ some environment of variable assignments) is
- defined by primitive recursion over the structure of expressions.
-*}
+text {* Evaluation (wrt.\ some environment of variable assignments) is
+  defined by primitive recursion over the structure of expressions. *}
 
-consts
-  eval :: "('adr, 'val) expr => ('adr => 'val) => 'val"
-
-primrec
+primrec eval :: "('adr, 'val) expr => ('adr => 'val) => 'val"
+where
   "eval (Variable x) env = env x"
-  "eval (Constant c) env = c"
-  "eval (Binop f e1 e2) env = f (eval e1 env) (eval e2 env)"
+| "eval (Constant c) env = c"
+| "eval (Binop f e1 e2) env = f (eval e1 env) (eval e2 env)"
 
 
 subsection {* Machine *}
 
-text {*
- Next we model a simple stack machine, with three instructions.
-*}
+text {* Next we model a simple stack machine, with three
+  instructions. *}
 
 datatype ('adr, 'val) instr =
-  Const 'val |
-  Load 'adr |
-  Apply "'val binop"
+    Const 'val
+  | Load 'adr
+  | Apply "'val binop"
 
-text {*
- Execution of a list of stack machine instructions is easily defined
- as follows.
-*}
-
-consts
-  exec :: "(('adr, 'val) instr) list
-    => 'val list => ('adr => 'val) => 'val list"
+text {* Execution of a list of stack machine instructions is easily
+  defined as follows. *}
 
 primrec
+  exec :: "(('adr, 'val) instr) list
+    => 'val list => ('adr => 'val) => 'val list"
+where
   "exec [] stack env = stack"
-  "exec (instr # instrs) stack env =
+| "exec (instr # instrs) stack env =
     (case instr of
       Const c => exec instrs (c # stack) env
     | Load x => exec instrs (env x # stack) env
     | Apply f => exec instrs (f (hd stack) (hd (tl stack))
                    # (tl (tl stack))) env)"
 
-definition execute :: "(('adr, 'val) instr) list => ('adr => 'val) => 'val" where
-  "execute instrs env == hd (exec instrs [] env)"
+definition
+  execute :: "(('adr, 'val) instr) list => ('adr => 'val) => 'val"
+  where "execute instrs env = hd (exec instrs [] env)"
 
 
 subsection {* Compiler *}
 
-text {*
- We are ready to define the compilation function of expressions to
- lists of stack machine instructions.
-*}
-
-consts
-  compile :: "('adr, 'val) expr => (('adr, 'val) instr) list"
+text {* We are ready to define the compilation function of expressions
+  to lists of stack machine instructions. *}
 
 primrec
+  compile :: "('adr, 'val) expr => (('adr, 'val) instr) list"
+where
   "compile (Variable x) = [Load x]"
-  "compile (Constant c) = [Const c]"
-  "compile (Binop f e1 e2) = compile e2 @ compile e1 @ [Apply f]"
+| "compile (Constant c) = [Const c]"
+| "compile (Binop f e1 e2) = compile e2 @ compile e1 @ [Apply f]"
 
 
-text {*
- The main result of this development is the correctness theorem for
- $\idt{compile}$.  We first establish a lemma about $\idt{exec}$ and
- list append.
-*}
+text {* The main result of this development is the correctness theorem
+  for @{text compile}.  We first establish a lemma about @{text exec}
+  and list append. *}
 
 lemma exec_append:
   "exec (xs @ ys) stack env =
@@ -146,13 +129,11 @@ proof -
 qed
 
 
-text {*
- \bigskip In the proofs above, the \name{simp} method does quite a lot
- of work behind the scenes (mostly ``functional program execution'').
- Subsequently, the same reasoning is elaborated in detail --- at most
- one recursive function definition is used at a time.  Thus we get a
- better idea of what is actually going on.
-*}
+text {* \bigskip In the proofs above, the @{text simp} method does
+  quite a lot of work behind the scenes (mostly ``functional program
+  execution'').  Subsequently, the same reasoning is elaborated in
+  detail --- at most one recursive function definition is used at a
+  time.  Thus we get a better idea of what is actually going on. *}
 
 lemma exec_append':
   "exec (xs @ ys) stack env = exec ys (exec xs stack env) env"
@@ -221,8 +202,7 @@ proof -
 
   have "execute (compile e) env = hd (exec (compile e) [] env)"
     by (simp add: execute_def)
-  also from exec_compile
-    have "exec (compile e) [] env = [eval e env]" .
+  also from exec_compile have "exec (compile e) [] env = [eval e env]" .
   also have "hd ... = eval e env" by simp
   finally show ?thesis .
 qed
